admitting some lemmas

experiments/test.v
@@ -6,51 +6,104 @@ Require Import ExtLib.Data.Monads.WriterMonad.
 
 Set Implicit Arguments.
 
+Section with_monad.
+  Import MonadNotation.
+  Local Open Scope monad_scope.
+
+  Definition FlagsT : Type := bool.
+
+  Variable Monoid_B : Monoid FlagsT.
+  Variable m : Type -> Type.
+  Context {Monad_m: Monad m}.
+  Context {Writer_m: MonadWriter Monoid_B m}.
+
+  Definition lift_uop
+             (op: nat -> nat)
+             (mx: m nat) : m nat :=
+    x <- mx ;;
+      tell (beq_nat x 0) ;;
+      ret (op x).
+
+  Definition lift_bop
+             (op: nat -> nat -> nat)
+             (mx my: m nat) : m nat :=
+    x <- mx ;; y <- my ;;
+      tell (orb (beq_nat x 0) (beq_nat y 0)) ;;
+      ret (op x y).
+End with_monad.
+
 Section WriterMonad.
   Variable s t : Type.
   Variable Monoid_s : Monoid s.
-  
+
   Definition writer := writerT Monoid_s ident.
   Definition runWriter x := unIdent (@runWriterT s Monoid_s ident t x).
   Definition execWriter x:= snd (runWriter x).
   Definition evalWriter x:= fst (runWriter x).
 End WriterMonad.
 
-Section with_monad.
-  Import MonadNotation.
-  Local Open Scope monad_scope.
-  
-  Definition FlagsT : Type := bool.
-  
-  Variable Monoid_B : Monoid FlagsT.
-  Variable m : Type -> Type.
-  Context {Monad_m: Monad m}.
-  Context {Writer_m: MonadWriter Monoid_B m}.
-  
-  Definition uop 
-             (op: nat -> nat)
-             (x: nat) : m nat :=
-    tell (beq_nat x 0) ;;
-         ret (op x).
-  
-  Definition bop 
-             (op: nat -> nat -> nat)
-             (x y: nat) : m nat :=
-    tell (orb (beq_nat x 0) (beq_nat y 0)) ;;
-         ret (op x y).
-End with_monad.
 
 Definition sticky := Build_Monoid orb false.
 Definition m : Type -> Type := writer sticky.
 
-Definition ex1 : m nat :=  bop plus 1 2.
-Definition ex2 : m nat :=  bop plus 0 5.
+Definition ex1 : m nat :=  (lift_bop plus) (ret 1) (ret 2).
+Definition ex2 : m nat :=  (lift_bop plus) (ret 0) (ret 5).
 
 Compute (runWriter ex1).
 Compute (execWriter ex1).
 Compute (evalWriter ex1).
 
 Compute (runWriter ex2).
+
+Definition equiv {T: Type} (a b: m T) :=
+  (evalWriter a) = (evalWriter b).
+
+Require Import Coq.Classes.Morphisms.
+
+Lemma evalWriter_lift_uop
+      (op: nat -> nat)
+      {a: m nat}
+  :
+    evalWriter (lift_uop op a) = op (evalWriter a).
+Proof.
+  reflexivity.
+Qed.
+
+Lemma evalWriter_lift_bop
+      (op: nat -> nat -> nat)
+      {a b: m nat}
+  :
+    evalWriter (lift_bop op a b) = op (evalWriter a) (evalWriter b).
+Proof.
+  reflexivity.
+Qed.
+
+Lemma test2
+      (op: nat -> nat)
+      `{op_mor: !Proper ((eq) ==> (eq)) op}
+      {a b: m nat}
+  :
+    equiv a b ->
+    equiv ((lift_uop op) a) ((lift_uop op) b).
+Proof.
+  intros H.
+
+  (*  Direct proof:
+  unfold equiv in *.
+  unfold evalWriter, runWriter in *.
+  unfold lift_uop.
+
+  simpl. (* also cbv or compute works *)
+  rewrite H.
+  reflexivity.
+   *)
+
+  unfold equiv in *.
+  rewrite 2!evalWriter_lift_uop.
+  rewrite H.
+  reflexivity.
+Qed.
+
 
 
 
